src/Internal/WfTuples.v
@@ -37,13 +37,6 @@ Variable lt: A -> A -> Prop.
 Variable wf_lt: well_founded lt.
 Local Infix "<" := lt.
 
-Definition lltlp := (clos_trans _ (WfMult.ltlp lt)).
-Definition wf_trans: well_founded lltlp.
-Proof.
-  apply wf_clos_trans. apply WfMult.wf_perm. apply wf_lt.
-Qed.
-
-
 (** 2 *)
 
 Definition le12 : A -> A * A -> Prop := fun a bs =>
@@ -57,20 +50,20 @@ Definition list2 {A: Type} := fun x: prod A A => let (x1, x2) := x in
   x1 :: x2 :: nil.
 
 Lemma le2lst:
-  forall x y, x << y -> other' lt (list2 x) (list2 y).
+  forall x y, x << y -> decr lt (list2 x) (list2 y).
 Proof.
   intros. destruct x, y.
   cut (forall a (b: list A), a :: b <> nil <-> True). intro Y.
-  destruct H, H, H0; simpl list2; rewrite other'_unfold; simpl; rewrite Y; tauto.
+  destruct H, H, H0; simpl list2; rewrite decr_unfold; simpl; rewrite Y; tauto.
   intros. pose proof (@nil_cons _ a3 b). clear wf_lt H. firstorder.
 Qed.
 
 Theorem wf_two: well_founded le22.
 Proof.
-  apply (wf_incl _ _ (fun x y => other' lt (list2 x) (list2 y))).
+  apply (wf_incl _ _ (fun x y => decr lt (list2 x) (list2 y))).
   unfold inclusion. apply le2lst.
-  apply (wf_inverse_image _ _ (other' lt) list2).
-  apply wf_other. assumption.
+  apply (wf_inverse_image _ _ (decr lt) list2).
+  apply wf_decr. assumption.
 Qed.
 
 Lemma wf_two_ind: forall P : A -> A -> Prop,
@@ -100,20 +93,20 @@ Definition list3 {A: Type} := fun x : A *A *A=>
   x1 :: x2 :: x3 :: nil end.
 
 Lemma le3lst:
-  forall x y, x <<< y -> other' lt (list3 x) (list3 y).
+  forall x y, x <<< y -> decr lt (list3 x) (list3 y).
 Proof.
   intros. destruct x, y, p, p0.
   cut (forall a (b: list A), a :: b <> nil <-> True). intro Y.
-  destruct H, H, H0, H0, H1; simpl list3; rewrite other'_unfold; simpl; rewrite Y; tauto.
+  destruct H, H, H0, H0, H1; simpl list3; rewrite decr_unfold; simpl; rewrite Y; tauto.
   intros. pose proof (@nil_cons _ a5 b). clear wf_lt H. firstorder.
 Qed.
 
 Theorem wf_three: well_founded le33.
 Proof.
-  apply (wf_incl _ _ (fun x y => other' lt (list3 x) (list3 y))).
+  apply (wf_incl _ _ (fun x y => decr lt (list3 x) (list3 y))).
   unfold inclusion. apply le3lst.
-  apply (wf_inverse_image _ _ (other' lt) list3).
-  apply wf_other. assumption.
+  apply (wf_inverse_image _ _ (decr lt) list3).
+  apply wf_decr. assumption.
 Qed.
 
 Lemma wf_three_ind:
